Updated typing rules

Typing.v
@@ -33,7 +33,8 @@ Definition kind := nat.
  *)
 Inductive tc_entry := 
   | TEtyping (_ : type * option size)
-  | TEkinding (_ : kind).
+  | TEkinding
+.
 
 Definition tcontext := list tc_entry.
 
@@ -41,28 +42,28 @@ Local Open Scope prog_scope.
 
 Definition add_typing t T := TEtyping t :: T.
 Definition add_typings ls T := fst $ fold_left (fun (p : tcontext * nat) t => let (T, n) := p in (add_typing (shiftby n t) T, S n)) ls (T, 0%nat).
-Definition add_kinding k T := TEkinding k :: T.
+Definition add_kinding T := TEkinding :: T.
 
 Coercion var_to_size (x : var) : size := Svar (x, []).
 
 Inductive kinding : tcontext -> type -> kind -> Prop :=
-| Kvar T n k : find n T = Some (TEkinding k) -> kinding T #n k
+| Kvar T x : find x T = Some TEkinding -> kinding T #x 0
 | Kapp T t1 t2 k :
     kinding T t1 (S k) ->
     kinding T t2 0 ->
     kinding T (Tapp t1 t2) k
 | Kabs T t k :
-    kinding (add_kinding 0 T) t k ->
+    kinding (add_kinding T) t k ->
     kinding T (Tabs t) (S k)
-| Karrow T t1 f g t2 :
+| Karrow T t1 c s t2 :
     kinding T t1 0 ->
     kinding (add_typing (t1, None) T) t2 0 ->
-    kinding T (Tarrow t1 f g t2) 0
-| Kuniversal T f g t :
-    kinding (add_kinding 0 T) t 0 ->
-    kinding T (Tuniversal f g t) 0
+    kinding T (Tarrow t1 c s t2) 0
+| Kuniversal T c s t :
+    kinding (add_kinding T) t 0 ->
+    kinding T (Tuniversal c s t) 0
 | Krecur T t :
-    kinding (add_kinding 0 T) t 0 ->
+    kinding (add_kinding T) t 0 ->
     kinding T (Trecur t) 0
 | Khide T t :
     kinding T t 0 ->
@@ -92,10 +93,10 @@ Inductive teq : type -> type -> Prop :=
     teq (Tapp a b) (Tapp a' b')
 | Qbeta t1 t2 :
     teq (Tapp (Tabs t1) t2) (subst t2 t1)
-| Qarrow a f g b a' b' : 
+| Qarrow a c s b a' b' : 
     teq a a' ->
     teq b b' ->
-    teq (Tarrow a f g b) (Tarrow a' f g b')
+    teq (Tarrow a c s b) (Tarrow a' c s b')
 | Qrecur a b :
     teq a b ->
     teq (Trecur a) (Trecur b)
@@ -137,52 +138,52 @@ Local Open Scope prog_scope.
 Notation Tuniversal0 := (Tuniversal F0 Stt).
 
 Inductive typing : tcontext -> expr -> type -> cexpr -> size -> Prop :=
-| TPvar T n t s : 
-    find n T = Some (TEtyping (t, s)) -> 
-    typing T #n (shiftby (S n) t) F0 (default (var_to_size #n) (shiftby (S n) s))
-| TPapp T e1 e2 ta tb n s n1 n2 nouse s2 : 
-    typing T e1 (Tarrow ta n s tb) n1 nouse ->
-    typing T e2 ta n2 s2 ->
-    typing T (Eapp e1 e2) (subst s2 tb) (n1 + n2 + F1 + subst s2 n) (subst s2 s)
-| TPabs T e t1 t2 n s :
+| TPvar T x t s : 
+    find x T = Some (TEtyping (t, s)) -> 
+    typing T #x (shiftby (S x) t) F0 (default (var_to_size #x) (shiftby (S x) s))
+| TPapp T e1 e2 ta tb c s c1 c2 nouse s2 : 
+    typing T e1 (Tarrow ta c s tb) c1 nouse ->
+    typing T e2 ta c2 s2 ->
+    typing T (Eapp e1 e2) (subst s2 tb) (c1 + c2 + subst s2 c) (subst s2 s)
+| TPabs T e t1 t2 c s :
     kinding T t1 0 ->
-    typing (add_typing (t1, None) T) e t2 n s ->
-    typing T (Eabs t1 e) (Tarrow t1 n s t2) F0 Stt
-| TPtapp T e t2 n s t n' :
-    typing T e (Tuniversal (shift n) (shift s) t) n' Stt ->
-    typing T (Etapp e t2) (subst t2 t) (n' + F1 + n) s
-| TPtabs T e n s t :
-    typing (add_kinding 0 T) e t n s ->
-    typing T (Etabs e) (Tuniversal n s t) F0 Stt
-| TPlet T t1 e1 e2 t2 n1 n2 s1 s2:
-    typing T e1 t1 n1 s1 ->
-    typing (add_typing (t1, Some s1) T) e2 t2 n2 s2 ->
-    typing T (Elet t1 e1 e2) (subst s1 t2) (n1 + subst s1 n2) (subst s1 s2)
-| TPfold T e t n s t1 :
+    typing (add_typing (t1, None) T) e t2 c s ->
+    typing T (Eabs t1 e) (Tarrow t1 c s t2) F0 Stt
+| TPtapp T e t2 c s t c' :
+    typing T e (Tuniversal (shift c) (shift s) t) c' Stt ->
+    typing T (Etapp e t2) (subst t2 t) (c' + c) s
+| TPtabs T e c s t :
+    typing (add_kinding T) e t c s ->
+    typing T (Etabs e) (Tuniversal c s t) F0 Stt
+| TPlet T t1 e1 e2 t2 c1 c2 s1 s2:
+    typing T e1 t1 c1 s1 ->
+    typing (add_typing (t1, Some s1) T) e2 t2 c2 s2 ->
+    typing T (Elet t1 e1 e2) (subst s1 t2) (c1 + subst s1 c2) (subst s1 s2)
+| TPfold T e t c s t1 :
     t == Trecur t1 ->
-    typing T e (subst t t1) n s ->
-    typing T (Efold t e) t n (Sfold s)
-| TPunfold T e t n s s1 t1 :
-    typing T e t n s ->
+    typing T e (subst t t1) c s ->
+    typing T (Efold t e) t c (Sfold s)
+| TPunfold T e t c s s1 t1 :
+    typing T e t c s ->
     is_fold s = Some s1 ->
     t == Trecur t1 ->
-    typing T (Eunfold e) (subst t t1) (1 + n) s1
-| TPhide T e t n s :
-    typing T e t n s ->
-    typing T (Ehide e) (Thide t) n (Shide s)
-| TPunhide T e t n s s1 :
-    typing T e (Thide t) n s ->
+    typing T (Eunfold e) (subst t t1) (F1 + c) s1
+| TPhide T e t c s :
+    typing T e t c s ->
+    typing T (Ehide e) (Thide t) c (Shide s)
+| TPunhide T e t c s s1 :
+    typing T e (Thide t) c s ->
     is_hide s = Some s1 ->
-    typing T (Eunhide e) t n s1
-| TPeq T e t1 t2 n s :
-    typing T e t1 n s ->
+    typing T (Eunhide e) t c s1
+| TPeq T e t1 t2 c s :
+    typing T e t1 c s ->
     t1 == t2 ->
-    typing T e t2 n s
-| TPsub T e t n n' s s' :
-    typing T e t n s ->
-    n <<= n' ->
+    typing T e t2 c s
+| TPsub T e t c c' s s' :
+    typing T e t c s ->
+    c <<= c' ->
     s <= s' ->
-    typing T e t n' s'
+    typing T e t c' s'
 (* basic types - intro *)
 | TPtt T :
     typing T Ett Tunit F0 Stt
@@ -197,29 +198,29 @@ Inductive typing : tcontext -> expr -> type -> cexpr -> size -> Prop :=
     typing T e te c s ->
     typing T (Einr t e) (Tsum t te) c (Sinr s)
 (* basic types - elim *)
-| TPmatch_pair T e e' t t1 t2 n s n' s' s1 s2 :
-    typing T e (Tprod t1 t2) n s ->
+| TPmatch_pair T e e' t t1 t2 c s c' s' s1 s2 :
+    typing T e (Tprod t1 t2) c s ->
     is_pair s = Some (s1, s2) ->
     let t12 := [(t1, Some s1); (t2, Some s2)] in
     let T' := add_typings t12 T in
-    typing T' e' t n' s' ->
+    typing T' e' t c' s' ->
     let s12 := [s1; s2] in
-    typing T (Ematch_pair e e') (subst_list s12 t) (n + F1 + subst_list s12 n') (subst_list s12 s')
-| TPmatch_inlinr T e e1 e2 t1 t2 n s s1 s2 t n1 n2 s' :
-    typing T e (Tsum t1 t2) n s ->
+    typing T (Ematch_pair e e') (subst_list s12 t) (c + subst_list s12 c') (subst_list s12 s')
+| TPmatch_inlinr T e e1 e2 t1 t2 c s s1 s2 t c1 c2 s' :
+    typing T e (Tsum t1 t2) c s ->
     is_inlinr s = Some (s1, s2) ->
     (* timing constraints are passed forward; size and type constraints are passed backward.
        t' and s' are backward guidance for branches *)
-    typing (add_typing (t1, Some s1) T) e1 (shift t) n1 (shift s') -> 
-    typing (add_typing (t2, Some s2) T) e2 (shift t) n2 (shift s') -> 
-    typing T (Ematch_sum e e1 e2) t (n + F1 + max (subst s1 n1) (subst s2 n2)) s'
-| TPmatch_inl T e e1 e2 t1 t2 n s t' n' s' :
-    typing T e (Tsum t1 t2) n (Sinl s) ->
-    typing (add_typing (t1, Some s) T) e1 t' n' s' ->
-    typing T (Ematch_sum e e1 e2) (subst s t') (n + F1 + subst s n') (subst s s')
-| TPmatch_inr T e e1 e2 t1 t2 n s t' n' s' :
-    typing T e (Tsum t1 t2) n (Sinr s) ->
-    typing (add_typing (t2, Some s) T) e2 t' n' s' ->
-    typing T (Ematch_sum e e1 e2) (subst s t') (n + F1 + subst s n') (subst s s')
+    typing (add_typing (t1, Some s1) T) e1 (shift t) c1 (shift s') -> 
+    typing (add_typing (t2, Some s2) T) e2 (shift t) c2 (shift s') -> 
+    typing T (Ematch_sum e e1 e2) t (c + max (subst s1 c1) (subst s2 c2)) s'
+| TPmatch_inl T e e1 e2 t1 t2 c s t' c' s' :
+    typing T e (Tsum t1 t2) c (Sinl s) ->
+    typing (add_typing (t1, Some s) T) e1 t' c' s' ->
+    typing T (Ematch_sum e e1 e2) (subst s t') (c + subst s c') (subst s s')
+| TPmatch_inr T e e1 e2 t1 t2 c s t' c' s' :
+    typing T e (Tsum t1 t2) c (Sinr s) ->
+    typing (add_typing (t2, Some s) T) e2 t' c' s' ->
+    typing T (Ematch_sum e e1 e2) (subst s t') (c + subst s c') (subst s s')
 .
 
