EvalCBV.v
@@ -22,23 +22,42 @@ Inductive IsValue : expr -> Prop :=
 
 (* evaluation context *)
 Inductive econtext :=
-  | ECempty
-  | ECapp1 (f : econtext) (arg : expr)
-  | ECapp2 (f : expr) (arg : econtext) : IsValue f -> econtext
-  | EClet (t : type) (def : econtext) (main : expr)
-  | ECtapp (f : econtext) (t : type)
-  | ECfold (t : type) (_ : econtext)
-  | ECunfold (_ : econtext)
-  | EChide (_ : econtext)
-  | ECunhide (_ : econtext)
-  | ECpair1 (a : econtext) (b : expr)
-  | ECpair2 (a : expr) (b : econtext) : IsValue a -> econtext
-  | ECinl (_ : type) (_ : econtext)
-  | ECinr (_ : type) (_ : econtext)
-  | ECmatch_pair (target : econtext) (_ : expr)
-  | ECmatch_sum (target : econtext) (a b : expr)
+| ECempty
+| ECapp1 (f : econtext) (arg : expr)
+| ECapp2 (f : expr) (arg : econtext) : IsValue f -> econtext
+| EClet (t : type) (def : econtext) (main : expr)
+| ECtapp (f : econtext) (t : type)
+| ECfold (t : type) (_ : econtext)
+| ECunfold (_ : econtext)
+| EChide (_ : econtext)
+| ECunhide (_ : econtext)
+| ECpair1 (a : econtext) (b : expr)
+| ECpair2 (a : expr) (b : econtext) : IsValue a -> econtext
+| ECinl (_ : type) (_ : econtext)
+| ECinr (_ : type) (_ : econtext)
+| ECmatch_pair (target : econtext) (_ : expr)
+| ECmatch_sum (target : econtext) (a b : expr)
 .
 
+Inductive plug : econtext -> expr -> expr -> Prop :=
+| Pempty e : plug ECempty e e
+| Papp1 E e f arg : plug E e f -> plug (ECapp1 E arg) e (Eapp f arg)
+| Papp2 E e arg f h : plug E e arg -> plug (ECapp2 f E h) e (Eapp f arg)
+| Plet E e def t main : plug E e def -> plug (EClet t E main) e (Elet t def main)
+| Ptapp E e f t : plug E e f -> plug (ECtapp E t) e (Etapp f t)
+| Pfold E e e' t : plug E e e' -> plug (ECfold t E) e (Efold t e')
+| Punfold E e e' : plug E e e' -> plug (ECunfold E) e (Eunfold e')
+| Phide E e e' : plug E e e' -> plug (EChide E) e (Ehide e')
+| Punhide E e e' : plug E e e' -> plug (ECunhide E) e (Eunhide e')
+| Ppair1 E e a b : plug E e a -> plug (ECpair1 E b) e (Epair a b)
+| Ppair2 E e b a h : plug E e b -> plug (ECpair2 a E h) e (Epair a b)
+| Pinl E e e' t : plug E e e' -> plug (ECinl t E) e (Einl t e')
+| Pinr E e e' t : plug E e e' -> plug (ECinr t E) e (Einr t e')
+| Pmatch_pair E e target k : plug E e target -> plug (ECmatch_pair E k) e (Ematch_pair target k)
+| Pmatch_sum E e target k1 k2 : plug E e target -> plug (ECmatch_sum E k1 k2) e (Ematch_sum target k1 k2)
+.
+
+(*
 Fixpoint plug (c : econtext) (e : expr) : expr :=
   match c with
     | ECempty => e
@@ -57,27 +76,32 @@ Fixpoint plug (c : econtext) (e : expr) : expr :=
     | ECmatch_pair target k => Ematch_pair (plug target e) k
     | ECmatch_sum target a b => Ematch_sum (plug target e) a b
   end.
+*)
 
 Inductive step : expr -> expr -> Prop :=
-  | STecontext c e1 e2 : step e1 e2 -> step (plug c e1) (plug c e2)
-  | STapp t body arg : IsValue arg -> step (Eapp (Eabs t body) arg) (subst arg body)
-  | STlet t v main : IsValue v -> step (Elet t v main) (subst v main)
-  | STmatch_pair ta tb a b k : 
-      IsValue a ->
-      IsValue b ->
-      step (Ematch_pair (Epair $$ ta $$ tb $$ a $$ b) k) (subst_list [a; b] k)
-  | STmatch_inl ta tb v k1 k2 : 
-      IsValue v ->
-      step (Ematch_sum (Einl $$ ta $$ tb $$ v) k1 k2) (subst v k1)
-  | STmatch_inr ta tb v k1 k2 : 
-      IsValue v ->
-      step (Ematch_sum (Einr $$ ta $$ tb $$ v) k1 k2) (subst v k2)
-  | STtapp body t : step (Etapp (Etabs body) t) (subst t body)
-  | STunfold_fold v t1 : 
-      IsValue v ->
-      step (Eunfold (Efold t1 v)) v
-  | STunhide_hide v :
-      IsValue v ->
-      step (Eunhide (Ehide v)) v
+| STecontext E e1 e2 e1' e2' : 
+    step e1 e2 -> 
+    plug E e1 e1' -> 
+    plug E e2 e2' -> 
+    step e1' e2'
+| STapp t body arg : IsValue arg -> step (Eapp (Eabs t body) arg) (subst arg body)
+| STlet t v main : IsValue v -> step (Elet t v main) (subst v main)
+| STmatch_pair t1 t2 v1 v2 k : 
+    IsValue v1 ->
+    IsValue v2 ->
+    step (Ematch_pair (Epair $$ t1 $$ t2 $$ v1 $$ v2) k) (subst_list [v1; v2] k)
+| STmatch_inl t1 t2 v k1 k2 : 
+    IsValue v ->
+    step (Ematch_sum (Einl $$ t1 $$ t2 $$ v) k1 k2) (subst v k1)
+| STmatch_inr t1 t2 v k1 k2 : 
+    IsValue v ->
+    step (Ematch_sum (Einr $$ t1 $$ t2 $$ v) k1 k2) (subst v k2)
+| STtapp body t : step (Etapp (Etabs body) t) (subst t body)
+| STunfold_fold v t1 : 
+    IsValue v ->
+    step (Eunfold (Efold t1 v)) v
+| STunhide_hide v :
+    IsValue v ->
+    step (Eunhide (Ehide v)) v
 .
 
